\documentclass[12pt]{article}
\usepackage{amsfonts}
\usepackage{fancyhdr}
\usepackage{comment}
\usepackage[letterpaper, top=2.5cm, bottom=2.5cm, left=2.2cm, right=2.2cm]%
{geometry}
\usepackage{amsmath}
\usepackage{changepage}
\usepackage{enumitem}
\usepackage{amssymb}
\usepackage{graphicx}
\usepackage{hyperref}

\newcommand{\cov}{\text{cov}}
\newcommand{\E}{\text{E}}

\begin{document}

    \title{SDS 383D Conditionals and Marginals}
    \author{Jan-Michael Cabrera, JC7858}
    \date{\today}
    \maketitle

    \section*{B: Inverse of the Covariance Matrix}

    Let $\Omega = \Sigma^{-1}$, partition $\Omega$ like $\Sigma$

    \begin{equation}
        \Omega = \begin{bmatrix} \Omega_{11} & \Omega_{12} \\ \Omega_{12}^T & \Omega_{22}\end{bmatrix}
    \end{equation}

    \begin{equation}
        \Sigma = \begin{bmatrix} \Sigma_{11} & \Sigma_{12} \\ \Sigma_{12}^T & \Sigma_{22}\end{bmatrix}
    \end{equation}

    \begin{equation}
        \Sigma \Omega = \begin{bmatrix} I & 0 \\ 0 & I \end{bmatrix}
    \end{equation}

    \begin{align}
        \Sigma \Omega & =\begin{bmatrix} \Sigma_{11} & \Sigma_{12} \\ \Sigma_{12}^T & \Sigma_{22}\end{bmatrix} \begin{bmatrix} \Omega_{11} & \Omega_{12} \\ \Omega_{12}^T & \Omega_{22}\end{bmatrix} \\
        &= \begin{bmatrix} \Sigma_{11} \Omega_{11}+ \Sigma_{12} \Omega_{12}^T & \Sigma_{11} \Omega_{12} + \Sigma_{12} \Omega_{22} \\ 
            \Sigma_{12}^T \Omega_{11} + \Sigma_{22}\Omega_{12}^T & \Sigma_{12}^T \Omega_{12} + \Sigma_{22} \Omega_{22}
        \end{bmatrix}
    \end{align}

    \begin{align}
        \Sigma_{11} \Omega_{11}+ \Sigma_{12} \Omega_{12}^T &= I\\
        \Sigma_{11} \Omega_{12} + \Sigma_{12} \Omega_{22} &= 0\\
        \Sigma_{12}^T \Omega_{11} + \Sigma_{22}\Omega_{12}^T &= 0\\
        \Sigma_{12}^T \Omega_{12} + \Sigma_{22} \Omega_{22} &= I
    \end{align}

    \begin{align}
        \Omega_{12} &= -\Sigma_{11}^{-1} \Sigma_{12}\Omega_{22} \\
        \Omega_{12}^T &= -\Sigma_{22}^{-1} \Sigma_{12}^T \Omega_{11}
    \end{align}

    \begin{equation}
        \Sigma_{11} \Omega_{11} + \Sigma_{12} ( -\Sigma_{22}^{-1} \Sigma_{12}^T \Omega_{11}) = (\Sigma_{11} - \Sigma_{12} \Sigma_{22}^{-1} \Sigma_{12}^T )\Omega_{11} =I
    \end{equation}

    \begin{equation}
        \Omega_{11} = (\Sigma_{11} - \Sigma_{12} \Sigma_{22}^{-1} \Sigma_{12}^T )^{-1}
    \end{equation}

    \begin{equation}
        \Sigma_{12}^T(-\Sigma_{11}^{-1} \Sigma_{12} \Omega_{22}) + \Sigma_{22} \Omega_{22} = (\Sigma_{22} - \Sigma_{12}^T \Sigma_{11}^{-1}\Sigma_{12})\Omega_{22} = I
    \end{equation}

    \begin{equation}
        \Omega_{22} = (\Sigma_{22} - \Sigma_{12}^T \Sigma_{11}^{-1}\Sigma_{12})^{-1}
    \end{equation}

    \begin{align}
        \Omega_{12} &= -\Sigma_{11}^{-1} \Sigma_{12}(\Sigma_{22} - \Sigma_{12}^T \Sigma_{11}^{-1}\Sigma_{12})^{-1} \\
        \Omega_{12}^T &= -\Sigma_{22}^{-1} \Sigma_{12}^T (\Sigma_{11} - \Sigma_{12} \Sigma_{22}^{-1} \Sigma_{12}^T )^{-1}
    \end{align}

    \begin{equation}
        \Omega = \Sigma^{-1} = \begin{bmatrix}
            (\Sigma_{11} - \Sigma_{12} \Sigma_{22}^{-1} \Sigma_{12}^T )^{-1} & -\Sigma_{11}^{-1} \Sigma_{12}(\Sigma_{22} - \Sigma_{12}^T \Sigma_{11}^{-1}\Sigma_{12})^{-1} \\
            -\Sigma_{22}^{-1} \Sigma_{12}^T (\Sigma_{11} - \Sigma_{12} \Sigma_{22}^{-1} \Sigma_{12}^T )^{-1} & (\Sigma_{22} - \Sigma_{12}^T \Sigma_{11}^{-1}\Sigma_{12})^{-1}
        \end{bmatrix}
    \end{equation}



\end{document}