\documentclass[12pt]{article}
\usepackage{amsfonts}
\usepackage{fancyhdr}
\usepackage{comment}
\usepackage[letterpaper, top=2.5cm, bottom=2.5cm, left=2.2cm, right=2.2cm]%
{geometry}
\usepackage{amsmath}
\usepackage{changepage}
\usepackage{enumitem}
\usepackage{amssymb}
\usepackage{graphicx}
\usepackage{hyperref}

\newcommand{\cov}{\text{cov}}
\newcommand{\E}{\text{E}}

\begin{document}

    \title{SDS 383D Conditionals and Marginals}
    \author{Jan-Michael Cabrera, JC7858}
    \date{\today}
    \maketitle

    \section*{C: Conditional Multivariate Normal}

        \begin{equation}
            p(x_1|x_2) = \frac{p(x_1, x_2)}{\int p(x_1, x_2) dx_1} \propto p(x_1, x_2)
        \end{equation}

        \begin{equation}
            p(x_1, x_2) \propto \text{exp} \left [ -\frac{1}{2} (x - \mu)^T \Sigma^{-1}(x - \mu)\right]
        \end{equation}

        \begin{align}
            & (x - \mu)^T \Sigma^{-1}(x - \mu) = \begin{bmatrix} (x_1 - \mu_1)^T, (x_2 - \mu_2)^T \end{bmatrix} \begin{bmatrix} \Omega_{11} & \Omega_{12} \\ \Omega_{12}^T & \Omega_{22} \end{bmatrix} \begin{bmatrix} (x_1 - \mu_1) \\ (x_2 - \mu_2) \end{bmatrix} \\
            & = \begin{bmatrix} (x_1 - \mu_1)^T \Omega_{11} + (x_2 - \mu_2)^T \Omega_{12}^T, (x_1 - \mu_1)^T \Omega_{12} + (x_2 - \mu_2)^T \Omega_{22} \end{bmatrix} \begin{bmatrix} (x_1 - \mu_1) \\ (x_2 - \mu_2)\end{bmatrix} \\
            & = ((x_1 - \mu_1)^T \Omega_{11} + (x_2 - \mu_2)^T \Omega_{12}^T)(x_1 - \mu_1) + ((x_1 - \mu_1)^T \Omega_{12} + (x_2 - \mu_2)^T \Omega_{22})(x_2 - \mu_2) \\
            & = (x_1 - \mu_1)^T \Omega_{11} (x_1 - \mu_1) + 2 (x_1 - \mu_1)^T \Omega_{12}^T (x_2 - \mu_2) + ...
        \end{align}

        \begin{equation}
            x^T A x + x^Tb = (x-h)^T A (x-h) + k \hspace{10pt} \text{where} \hspace{10pt} h = -\frac{1}{2}A^{-1}b \hspace{10pt} \text{and} \hspace{10pt} k = -\frac{1}{4}b^T A^{-1} b
        \end{equation}

        \begin{align}
            & (x_1 - \mu_1)^T A (x_1 - \mu_1) + (x_1 - \mu_1) b = (x_1 - \mu_1 - h)^T A (x_1 - \mu_1 - h) + ... \\
            & \text{where} \hspace{10pt} A = \Sigma_{11} \hspace{10pt} \text{and} \hspace{10pt} b = 2 \Sigma_{12}^T (x_2 - \mu_2)
        \end{align}

        \begin{align}
            h &= -\frac{1}{2}A^{-1}b = -\frac{1}{2}\Omega_{11}^{-1}2 \Omega_{12} (x_2 - \mu_2) \\
            & = -\Omega_{11}^{-1}\Omega_{12}^T (x_2 - \mu_2) \hspace{10pt} \text{where} \hspace{10pt} \Omega_{12}^T = -\Sigma_{22}^{-1} \Sigma_{12}^T \Omega_{11} \\
            & = \Sigma_{22}^{-1} \Sigma_{12}^T (x_2 - \mu_2)
        \end{align}

        \begin{equation}
            (x_1 - \mu_1 - h)^T A (x_1 - \mu_1 - h) = (x_1 - \mu^*)^T \Sigma_{11}^* (x_1 - \mu^*)
        \end{equation}

        \begin{align}
            \mu^* = \mu_1 + \Sigma_{22}^{-1} \Sigma_{12}^T(x_2 - \mu_2) \\
            \Sigma_{11}^* = \Omega_{11}^{-1} = \Sigma_{11} - \Sigma_{12} \Sigma_{22}^{-1} \Sigma_{12}^T
        \end{align}

        \begin{equation}
            x_1 | x_2 \sim \text{N}(\mu_1 + \Sigma_{22}^{-1} \Sigma_{12}^T(x_2 - \mu_2), \Sigma_{11} - \Sigma_{12} \Sigma_{22}^{-1}\Sigma_{12}^T)
        \end{equation}

\end{document}