\documentclass[12pt]{article}
\usepackage{amsfonts}
\usepackage{fancyhdr}
\usepackage{comment}
\usepackage[letterpaper, top=2.5cm, bottom=2.5cm, left=2.2cm, right=2.2cm]%
{geometry}
\usepackage{amsmath}
\usepackage{changepage}
\usepackage{enumitem}
\usepackage{amssymb}
\usepackage{graphicx}
\usepackage{hyperref}

\begin{document}

    \title{SDS 383D The Multivariate Normal Distribution}
    \author{Jan-Michael Cabrera, JC7858}
    \date{\today}
    \maketitle

    \section*{F: Multivariate Normal PDF}

        \begin{equation}
            f_Z(z) = \left ( \frac{1}{\sqrt{2 \pi}}\right)^{1/n} \text{exp} \left [ -\frac{1}{2} z^T z\right]
        \end{equation}

        \begin{equation}
            x = Lz + \mu, \hspace{20pt} z = L^{-1}(x - \mu)
        \end{equation}

        \begin{align}
            f_X(x) &= f_Z(h(z))\cdot|\text{det}(\nabla h(z))| \\
            &= f_Z(L^{-1}(x-\mu)) \cdot |\text{det}(L^{-1})| \\
            &= \left( \frac{1}{\sqrt{2 \pi}}\right) \text{exp}\left[ -\frac{1}{2}(L^{-1}(x-\mu))^T (L^{-1}(x-\mu))\right]\cdot |\text{det}(L^{-1})| \\
            &= \left( \frac{1}{\sqrt{2 \pi}}\right) \text{exp}\left[ -\frac{1}{2}(x-\mu)^T (L^{-1})^T L^{-1}(x-\mu)\right]\cdot |\text{det}(L^{-1})|
        \end{align}

        \begin{equation}
            |\text{det}(L^{-1})| = \frac{1}{\sqrt{\text{det}L^T L}}, \hspace{20pt}(L^T)^{-1} = (L^{-1})^T, \hspace{20pt} L^TL = \Sigma
        \end{equation}

        \begin{equation}
            f_X(x) = \left ( \frac{1}{\sqrt{2 \pi}}\right)^{1/n} \frac{1}{\sqrt{\text{det}\Sigma}} \text{exp} \left [ -\frac{1}{2} (x-\mu)^T \Sigma^{-1} (x-\mu)\right]
        \end{equation}

\end{document}